Applying a concept of using local (transactional) and global invariants to the example.

src/Blocking.v
@@ -1,7 +1,13 @@
+Require Import Common.
 Require Import Syntax Semantics StepDet.
 
 (* Below we describe a semantic interpretation of a system which has a
  * blocking property.
+ *
+ * There can be some static conditions for a target [System] to be [Blocking], 
+ * for instance, each rule handling messages from a specific external channel 
+ * has its own flag to block additional messages from the channel when it is
+ * currently handling a certain message from that channel.
  *)
 
 (* A message pool [msgs] is [Blocked] if any two messages in [msgs] whose 
@@ -16,8 +22,11 @@ Definition Blocked (msgs: Messages TMsg) :=
     InM m1 msgs -> InM m2 msgs ->
     tmsg_info m1 = Some ti1 ->
     tmsg_info m2 = Some ti2 ->
-    tinfo_rqin ti1 ≡m tinfo_rqin ti2 ->
+    mid_addr (msg_id (tinfo_rqin ti1)) = mid_addr (msg_id (tinfo_rqin ti2)) ->
     ti1 = ti2.
+
+Definition BlockedInv (tst: TState) :=
+  Blocked (tst_msgs tst).
 
 (* When two messages in the same channel are handled, [steps_det] ensures that 
  * the two messages have different [tinfo_tid]s. Thus, if a target [System] has 
@@ -28,9 +37,21 @@ Definition Blocking (sys: System) :=
     Reachable steps_det sys st ->
     Blocked (tst_msgs st).
 
-(* There are some static conditions for a target [System] to be [Blocking], for
- * instance, each rule handling messages from a specific external channel has
- * its own flag to block additional messages from the channel when it is 
- * currently handling a certain message from that channel.
- *)
+Require Import TrsSim.
+
+Section Facts.
+
+  Lemma BlockedInv_in:
+    forall sys, TrsSimSepGInvIn BlockedInv sys.
+  Proof.
+    unfold TrsSimSepGInvIn; intros.
+    inv H0.
+    unfold BlockedInv, Blocked in *; simpl in *; intros.
+  Admitted.
+
+  (* TODO: define a simulation for {impl, spec} messages;
+   * prove [Blocked .. -> Simulation .. -> (relation between [firstM])
+   *)
+
+End Facts.
 
